prove spec for free_body !

theories/iris/allocator/blocks.v
@@ -55,5 +55,3 @@ Definition final_block_addr (blk: final_block) : N :=
   match blk with
   | FinalBlk addr _ => addr
   end.
-
-Definition blocks := gmap 
